cedar-lean/Cedar/Thm/Data/Map.lean
@@ -27,19 +27,125 @@ This file proves useful properties of canonical list-based maps defined in
 
 namespace Cedar.Data.Map
 
-/-! ### Well-formed sets -/
+/-! ### Well-formed maps -/
 
 def WellFormed {α β} [LT α] [DecidableLT α] (m : Map α β) :=
   m = Map.make m.toList
 
-/-! ### contains and mem -/
+/--
+  In well-formed maps, if there are two pairs with the same key, then they have
+  the same value
+-/
+theorem key_maps_to_one_value [BEq α] [LT α] [DecidableLT α] (k : α) (v₁ v₂ : β) (m : Map α β) :
+  m.WellFormed →
+  (k, v₁) ∈ m.kvs →
+  (k, v₂) ∈ m.kvs →
+  v₁ = v₂
+:= by
+  unfold WellFormed toList
+  intro wf h₁ h₂
+  sorry
 
-theorem in_list_in_map {α : Type u} (k : α) (v : β) (m : Map α β) :
+/--
+  In well-formed maps, if a key maps to a value, then all equal keys (by BEq)
+  also map to that value
+-/
+theorem equal_keys_same_value [BEq α] [LT α] [DecidableLT α] (k₁ k₂ : α) (v : β) (m : Map α β) :
+  m.WellFormed →
+  (k₁, v) ∈ m.kvs →
+  k₁ == k₂ →
+  (k₂, v) ∈ m.kvs
+:= by
+  unfold WellFormed toList
+  intro wf h₁ h₂
+  sorry
+
+/--
+  `make` on equivalent lists of (k,v) pairs produces equal maps
+
+  (Organizationally belongs in the `make` section, but is needed before that)
+-/
+theorem make_eqv [LT α] [DecidableLT α] {xs ys : List (α × β)}:
+  xs ≡ ys →
+  Map.make xs = Map.make ys
+:= by
+  unfold make
+  intro h₁
+  sorry
+
+/--
+  If two well-formed maps have equivalent (k,v) sets, then the maps are actually
+  equal
+-/
+theorem eq_iff_kvs_equiv [LT α] [DecidableLT α] {m₁ m₂ : Map α β}
+  (wf₁ : m₁.WellFormed)
+  (wf₂ : m₂.WellFormed) :
+  m₁.kvs ≡ m₂.kvs ↔ m₁ = m₂
+:= by
+  constructor
+  case mp =>
+    intro h₁
+    unfold WellFormed toList at wf₁ wf₂
+    rw [wf₁]
+    rw [wf₂]
+    exact make_eqv h₁
+  case mpr =>
+    intro h₁
+    subst h₁
+    exact List.Equiv.refl
+
+/-! ### contains, mem, and find? -/
+
+theorem in_list_in_map {α : Type u} {k : α} {v : β} {m : Map α β} :
   (k, v) ∈ m.kvs → k ∈ m
 := by
   intro h₀
   have h₁ : k ∈ (List.map Prod.fst m.kvs) := by simp only [List.mem_map] ; exists (k, v)
   apply h₁
+
+theorem in_kvs_snd_in_values {kv : α × β} {m : Map α β} :
+  kv ∈ m.kvs → kv.snd ∈ m.values
+:= by
+  simp only [values, List.mem_map]
+  intro h₁
+  exists kv
+
+theorem in_list_some_find? [DecidableEq α] [LT α] [DecidableLT α] {k : α} {v : β} {m : Map α β} :
+  m.WellFormed →
+  ((k, v) ∈ m.kvs ↔ m.find? k = some v)
+:= by
+  intro h₁
+  unfold find?
+  constructor
+  case mp =>
+    intro h₂
+    cases h₃ : m.kvs.find? λ x => match x with | (k', _) => k' == k
+    case none =>
+      exfalso
+      rw [List.find?_eq_none] at h₃
+      specialize h₃ (k, v) h₂
+      apply h₃ ; clear h₃
+      simp
+    case some kv =>
+      simp only [Option.some.injEq]
+      have h₄ := List.find?_some h₃
+      simp only [beq_iff_eq] at h₄
+      subst h₄
+      replace h₃ := List.mem_of_find?_eq_some h₃
+      apply (key_maps_to_one_value kv.fst v kv.snd m h₁ h₂ _).symm
+      trivial
+  case mpr =>
+    intro h₂
+    cases h₃ : m.kvs.find? λ x => match x with | (k', _) => k' == k
+    case none => simp [h₃] at h₂
+    case some kv =>
+      simp only [h₃, Option.some.injEq] at h₂
+      subst h₂
+      have h₄ := List.mem_of_find?_eq_some h₃
+      replace h₃ := List.find?_some h₃
+      split at h₃ ; rename_i k' v
+      simp only
+      exact equal_keys_same_value k' k v m h₁ h₄ h₃
 
 theorem contains_iff_some_find? {α β} [BEq α] {m : Map α β} {k : α} :
   m.contains k ↔ ∃ v, m.find? k = .some v
@@ -54,76 +160,308 @@ theorem not_contains_of_empty {α β} [BEq α] (k : α) :
 theorem make_wf [LT α] [StrictLT α] [DecidableLT α] (xs : List (α × β)) :
   WellFormed (Map.make xs)
 := by
-  simp only [WellFormed, make, toList, kvs, List.canonicalize_idempotent]
+  simp [WellFormed, make, toList, kvs, List.canonicalize_idempotent]
 
-theorem make_mem_list_mem [LT α] [StrictLT α] [DecidableLT α] {xs : List (α × β)} :
+/-
+  Note that the converse of this is not true:
+  counterexample `xs = [(1, false), (1, true)]`.
+  Then `Map.make xs = [(1, false)]`.
+-/
+theorem mem_kvs_make [LT α] [StrictLT α] [DecidableLT α] {xs : List (α × β)} :
   x ∈ (Map.make xs).kvs → x ∈ xs
 := by
   simp only [kvs, make]
   intro h₁
   have h₂ := List.canonicalize_subseteq Prod.fst xs
-  simp [List.subset_def] at h₂
+  simp only [List.subset_def] at h₂
   exact h₂ h₁
+
+/--
+  Very similar to `mem_kvs_make` above
+-/
+theorem mem_values_make [LT α] [StrictLT α] [DecidableLT α] {xs : List (α × β)} :
+  v ∈ (Map.make xs).values → v ∈ xs.map Prod.snd
+:= by
+  -- despite the similarity to `mem_kvs_make`, the proof does not currently
+  -- use `mem_kvs_make`
+  simp only [values, make]
+  simp only [List.mem_map, forall_exists_index, and_imp]
+  intro (k, v) h₁ h₂
+  exists (k, v)
+  subst h₂
+  simp only [and_true]
+  have h₂ := List.canonicalize_subseteq Prod.fst xs
+  simp only [List.subset_def] at h₂
+  exact @h₂ (k, v) h₁
 
 theorem make_nil_is_empty {α β} [LT α] [DecidableLT α] :
   (Map.make [] : Map α β) = Map.empty
 := by simp [make, empty, List.canonicalize_nil]
 
+/--
+  Note that the converse of this is not true:
+  counterexample `xs = [(1, false)]`, `ys = []`, `ab = (1, false)`.
+-/
+theorem make_cons [LT α] [DecidableLT α] {xs ys : List (α × β)} {ab : α × β} :
+  make xs = make ys → make (ab :: xs) = make (ab :: ys)
+:= by
+  simp only [make, mk.injEq]
+  apply List.canonicalize_cons
+
 /-! ### find? and mapOnValues -/
 
-theorem find?_mapOnValues {α β γ} [LT α] [DecidableLT α] [DecidableEq α] (f : β → γ) (m : Map α β) (k : α)  :
+theorem mapOnValues_wf [LT α] [DecidableLT α] [DecidableEq α] {f : β → γ} {m : Map α β} :
+  m.WellFormed ↔ (m.mapOnValues f).WellFormed
+:= by
+  unfold mapOnValues WellFormed toList
+  sorry
+
+theorem mapOnValues_empty {α β γ} [LT α] [DecidableLT α] [DecidableEq α] {f : β → γ} :
+  (empty : Map α β).mapOnValues f = empty
+:= by
+  simp [mapOnValues, empty]
+
+theorem find?_mapOnValues {α β γ} [LT α] [DecidableLT α] [DecidableEq α] {f : β → γ} {m : Map α β} {k : α}  :
   (m.find? k).map f = (m.mapOnValues f).find? k
 := by
-  simp [Map.find?, Map.mapOnValues, Map.kvs, ←List.find?_pair_map]
-  cases __ : List.find? (fun x => x.fst == k) m.1 <;>
-  simp only [Option.map_none', Option.map_some']
+  simp only [find?, kvs, mapOnValues, ← List.find?_pair_map]
+  cases m.1.find? (λ x => x.fst == k) <;> simp
 
-theorem find?_mapOnValues_some {α β γ} [LT α] [DecidableLT α] [DecidableEq α] (f : β → γ) {m : Map α β} {k : α} {v : β} :
+theorem find?_mapOnValues_some {α β γ} [LT α] [DecidableLT α] [DecidableEq α] {f : β → γ} {m : Map α β} {k : α} {v : β} :
   m.find? k = .some v →
   (m.mapOnValues f).find? k = .some (f v)
 := by
   intro h₁
-  rw [← find?_mapOnValues f m k]
+  rw [← find?_mapOnValues]
   simp [Option.map, h₁]
 
-theorem find?_mapOnValues_none {α β γ} [LT α] [DecidableLT α] [DecidableEq α] (f : β → γ) {m : Map α β} {k : α} :
+theorem find?_mapOnValues_none {α β γ} [LT α] [DecidableLT α] [DecidableEq α] {f : β → γ} {m : Map α β} {k : α} :
   m.find? k = .none →
   (m.mapOnValues f).find? k = .none
 := by
   intro h₁
-  rw [← find?_mapOnValues f m k]
+  rw [← find?_mapOnValues]
   simp [Option.map, h₁]
 
-theorem mapOnValues_eq_make_map {α β γ} [LT α] [StrictLT α] [DecidableLT α] (f : β → γ) {m : Map α β}
-  (h₁ : m.WellFormed) :
+theorem mapOnValues_eq_make_map {α β γ} [LT α] [StrictLT α] [DecidableLT α] {f : β → γ} {m : Map α β}
+  (wf : m.WellFormed) :
   m.mapOnValues f = Map.make (m.toList.map λ kv => (kv.fst, f kv.snd))
 := by
-  simp [Map.WellFormed] at h₁
-  simp [Map.mapOnValues, Map.toList, Map.kvs, Map.make] at *
-  rw [h₁] ; simp only ; rw [eq_comm]
-  have h₂ : Prod.map id f = (fun (x : α × β) => (x.fst, f x.snd)) := by unfold Prod.map ; simp only [id_eq]
-  simp only [← h₂, ← List.canonicalize_of_map_fst, List.canonicalize_idempotent]
+  unfold WellFormed at wf
+  simp only [make, toList, kvs, mapOnValues, mk.injEq] at *
+  rw [wf] ; simp only ; rw [eq_comm]
+  have h₁ : Prod.map id f = (λ (x : α × β) => (x.fst, f x.snd)) := by unfold Prod.map ; simp only [id_eq]
+  simp only [← h₁, ← List.canonicalize_of_map_fst, List.canonicalize_idempotent]
 
-theorem find?_mem_toList {α β} [LT α] [DecidableLT α] [DecidableEq α] {m : Map α β} {k : α} {v : β}
-  (h₁ : m.find? k = .some v) :
-  (k, v) ∈ m.toList
-:= by
-  simp [Map.toList, Map.kvs, Map.find?] at *
-  split at h₁ <;> simp at h₁
-  subst h₁
-  rename_i h₂
-  have h₃ := List.find?_some h₂
-  simp at h₃ ; subst h₃
-  exact List.mem_of_find?_eq_some h₂
-
-theorem mapOnValues_contains {α β γ} [LT α] [DecidableLT α] [DecidableEq α] (f : β → γ) {m : Map α β} {k : α} :
+theorem mapOnValues_contains {α β γ} [LT α] [DecidableLT α] [DecidableEq α] {f : β → γ} {m : Map α β} {k : α} :
   Map.contains m k = Map.contains (Map.mapOnValues f m) k
 := by
   simp only [contains, Option.isSome]
   split
-  case h_1 h => simp [find?_mapOnValues_some f h]
-  case h_2 h => simp [find?_mapOnValues_none f h]
+  case h_1 h => simp [find?_mapOnValues_some h]
+  case h_2 h => simp [find?_mapOnValues_none h]
 
+theorem values_mapOnValues [LT α] [StrictLT α] [DecidableLT α] [DecidableEq α] {f : β → γ} {m : Map α β} :
+  (m.mapOnValues f).values = m.values.map f
+:= by
+  unfold mapOnValues values kvs
+  induction m.1
+  case nil => simp
+  case cons hd tl ih =>
+    simp only [List.map_cons, List.cons.injEq, true_and]
+    trivial
+
+theorem findOrErr_mapOnValues [LT α] [DecidableLT α] [DecidableEq α] {f : β → γ} {m : Map α β} {k : α} {e : Error} :
+  (m.mapOnValues f).findOrErr k e = (m.findOrErr k e).map f
+:= by
+  unfold findOrErr
+  rw [← find?_mapOnValues]
+  cases m.find? k <;> simp [Except.map]
+
+theorem findOrErr_ok_iff_find?_some [LT α] [DecidableLT α] [DecidableEq α] {m : Map α β} {k : α} {v : β} {e : Error} :
+  m.findOrErr k e = .ok v ↔ m.find? k = some v
+:= by
+  unfold findOrErr
+  cases m.find? k <;> simp
+
+theorem in_values_iff_findOrErr_ok [LT α] [DecidableLT α] [DecidableEq α] {m : Map α β} {v : β} {e : Error}
+  (wf : m.WellFormed) :
+  v ∈ m.values ↔ ∃ k, m.findOrErr k e = .ok v
+:= by
+  simp only [values, List.mem_map, findOrErr_ok_iff_find?_some]
+  constructor
+  case mp =>
+    intro h₁
+    replace ⟨⟨k, v'⟩, ⟨h₁, h₂⟩⟩ := h₁
+    simp only at h₂
+    subst v'
+    exists k
+    simp [h₁, ← in_list_some_find? wf]
+  case mpr =>
+    intro h₁
+    replace ⟨k, h₁⟩ := h₁
+    exists (k, v)
+    simp [h₁, in_list_some_find? wf, and_true]
+
+theorem in_kvs_in_mapOnValues [LT α] [DecidableLT α] [DecidableEq α] {f : β → γ} {m : Map α β} {k : α} {v : β} :
+  (k, v) ∈ m.kvs → (k, f v) ∈ (m.mapOnValues f).kvs
+:= by
+  unfold mapOnValues
+  intro h₁
+  simp only [kvs, List.mem_map, Prod.mk.injEq]
+  exists (k, v)
+
+/-! ### mapMOnValues -/
+
+theorem mapMOnValues_wf [LT α] [DecidableLT α] {f : β → Option γ} {m₁ : Map α β} {m₂ : Map α γ} :
+  m₁.WellFormed →
+  (m₁.mapMOnValues f = some m₂) →
+  m₂.WellFormed
+:= by
+  unfold WellFormed toList
+  intro wf h₁
+  simp only [mapMOnValues, Option.pure_def, Option.bind_eq_bind, Option.bind_eq_some,
+    Option.some.injEq] at h₁
+  replace ⟨xs, h₁, h₂⟩ := h₁
+  subst h₂
+  sorry
+
+/--
+  Isolating the lemma needed for `isSome_mapMOnValues`, which I'm having trouble
+  proving as of this writing.
+  Once proved, we can decide whether we actually want this stated as a separate
+  lemma or just inline the proof into `isSome_mapMOnValues`.
+-/
+theorem lemma {f : β → Option γ} {abs : List (α × β)} {ags : List (α × γ)} :
+  abs.mapM (λ ab => (f ab.snd).bind λ g => some (ab.fst, g)) = some ags →
+  (abs.map Prod.snd).mapM f = ags.map Prod.snd
+:= by
+  intro h₁
+  induction abs
+  case nil => simp only [List.mapM_nil, Option.pure_def, Option.some.injEq] at h₁ ; subst h₁ ; simp
+  case cons hd tl ih => -- this isn't the statement of `ih` that I want. Somehow we need to induction on both `abs` and `ags` simultaneously. We know they're the same length from `h₁`.
+    have (a, b) := hd ; clear hd
+    replace ⟨h₁, _⟩ := List.mapM_eq_some h₁
+    simp only [List.mem_cons, Option.bind_eq_some, Option.some.injEq, forall_eq_or_imp] at h₁
+    replace ⟨⟨(a', g), h₁, ⟨g', h₂, h₃⟩⟩, h₄⟩ := h₁
+    simp only [Prod.mk.injEq] at h₃
+    replace ⟨h₃, h₃'⟩ := h₃
+    subst h₃ h₃'
+    sorry
+
+/--
+  Analogue of `List.isSome_mapM` for Map.mapMOnValues
+-/
+theorem isSome_mapMOnValues [LT α] [DecidableLT α] {f : β → Option γ} {m : Map α β} :
+  Option.isSome (m.mapMOnValues f) ↔ ∀ v ∈ m.values, Option.isSome (f v)
+:= by
+  unfold Map.mapMOnValues
+  constructor
+  case mp =>
+    intro h₁
+    apply (List.isSome_mapM (xs := m.values)).mp
+    replace ⟨m', h₁⟩ := Option.isSome_iff_exists.mp h₁
+    rw [Option.isSome_iff_exists]
+    exists m'.values
+    cases h₂ : m.kvs.mapM (λ x => match x with | (k, v) => do let v' ← f v ; pure (k, v'))
+    <;> simp only [Option.pure_def, Option.bind_eq_bind, Option.bind_eq_some, Option.some.injEq] at h₁
+    <;> replace ⟨ags, h₁, h₃⟩ := h₁
+    <;> subst h₃
+    case some xs' =>
+      simp only [values]
+      apply lemma (f := f) (abs := m.kvs) h₁
+    case none =>
+      exfalso
+      replace ⟨(k, v), h₂, h₃⟩ := List.mapM_eq_none.mp h₂
+      simp only [Option.pure_def, Option.bind_eq_bind, Option.bind_eq_none] at h₃
+      replace h₁ := (Option.isSome_iff_exists (x := m.kvs.mapM λ x => (f x.snd).bind λ v => some (x.fst, v))).mpr (by exists ags)
+      rw [List.isSome_mapM] at h₁
+      specialize h₁ (k, v) h₂
+      simp only [Option.isSome, Option.bind] at h₁
+      cases h₄ : f v
+      case some => simp [h₄] at h₃
+      case none => simp [h₄] at h₁
+  case mpr =>
+    intro h₁
+    cases h₂ : m.kvs.mapM (λ x => match x with | (k, v) => do let v' ← f v ; pure (k, v'))
+    <;> simp only [Option.pure_def, Option.bind_none_fun, Option.bind_some_fun, Option.isSome_none, Option.isSome_some]
+    case none =>
+      replace ⟨(k, v), h₂, h₃⟩ := List.mapM_eq_none.mp h₂
+      specialize h₁ v (Map.in_kvs_snd_in_values h₂)
+      cases h₄ : f v
+      case some => simp [h₄] at h₃
+      case none => simp [h₄] at h₁
+
+/--
+  Analogue of `List.mapM_eq_none` for Map.mapMOnValues
+
+  Corollary of `isSome_mapMOnValues`
+-/
+theorem mapMOnValues_eq_none [LT α] [DecidableLT α] {f : β → Option γ} {m : Map α β} :
+  m.mapMOnValues f = none ↔ ∃ v ∈ m.values, f v = none
+:= by
+  -- As of this writing, this proof is nearly syntactically identical to the
+  -- proof of `List.mapM_eq_none`
+  constructor
+  case mp =>
+    intro h₁
+    by_contra h₂
+    replace h₂ := forall_not_of_not_exists h₂
+    simp only [not_and] at h₂
+    rw [← Option.not_isSome_iff_eq_none] at h₁
+    rw [isSome_mapMOnValues] at h₁
+    apply h₁ ; clear h₁
+    intro v h₁
+    specialize h₂ v h₁
+    rw [← ne_eq] at h₂
+    rw [Option.ne_none_iff_isSome] at h₂
+    exact h₂
+  case mpr =>
+    intro h₁
+    replace ⟨v, h₁, h₂⟩ := h₁
+    rw [← Option.not_isSome_iff_eq_none]
+    intro h₃
+    rw [isSome_mapMOnValues] at h₃
+    specialize h₃ v h₁
+    simp [h₂] at h₃
+
+/--
+  Analogue of `List.mapM_eq_some` for Map.mapMOnValues
+-/
+theorem mapMOnValues_eq_some [LT α] [DecidableLT α] {f : β → Option γ} {m₁ : Map α β} {m₂ : Map α γ} :
+  (m₁.mapMOnValues f = some m₂) → (
+    (∀ kv ∈ m₁.kvs, ∃ v, (kv.fst, v) ∈ m₂.kvs ∧ f kv.snd = some v) ∧
+    (∀ kv ∈ m₂.kvs, ∃ v, (kv.fst, v) ∈ m₁.kvs ∧ f v = kv.snd)
+  )
+:= by
+  unfold mapMOnValues
+  intro h₁
+  constructor
+  <;> intro kv h₂
+  <;> cases h₃ : m₁.kvs.mapM (λ x => match x with | (k, v) => do let v' ← f v ; pure (k, v'))
+  <;> rw [h₃] at h₁
+  <;> simp only [Option.pure_def, Option.bind_some_fun, Option.bind_none_fun, Option.some.injEq] at h₁
+  <;> subst h₁
+  case left.some ags =>
+    have (a, b) := kv ; clear kv
+    simp only
+    replace ⟨h₃, _⟩ := List.mapM_eq_some h₃
+    replace ⟨(a', g), h₃, h₄⟩ := h₃ (a, b) h₂
+    simp only [Option.pure_def, Option.bind_eq_bind, Option.bind_eq_some, Option.some.injEq,
+      Prod.mk.injEq, exists_eq_right_right] at h₄
+    replace ⟨h₄, h₄'⟩ := h₄
+    subst a'
+    exists g
+  case right.some ags =>
+    have (a, g) := kv ; clear kv
+    simp only
+    replace ⟨_, h₃⟩ := List.mapM_eq_some h₃
+    replace ⟨(a', b), h₃, h₄⟩ := h₃ (a, g) h₂
+    simp only [Option.pure_def, Option.bind_eq_bind, Option.bind_eq_some, Option.some.injEq,
+      Prod.mk.injEq, exists_eq_right_right] at h₄
+    replace ⟨h₄, h₄'⟩ := h₄
+    subst a'
+    exists b
 
 /-! ### sizeOf -/
 
@@ -133,13 +471,12 @@ theorem sizeOf_lt_of_value [SizeOf α] [SizeOf β] {m : Map α β} {k : α} {v :
 := by
   simp only [Membership.mem] at h
   replace h := List.sizeOf_lt_of_mem h
-  have _ : sizeOf v < sizeOf (k, v) := by
+  have v_lt_kv : sizeOf v < sizeOf (k, v) := by
     simp only [sizeOf, Prod._sizeOf_1]
     omega
-  have _ : sizeOf m.1 < sizeOf m := by
+  have m1_lt_m : sizeOf m.1 < sizeOf m := by
     simp only [sizeOf, _sizeOf_1]
     omega
-  rename_i v_lt_kv m1_lt_m
   let a := sizeOf v
   let c := sizeOf m.1
   let d := sizeOf m
