cedar-lean/Cedar/Thm/Partial/Evaluation/And.lean
@@ -1,0 +1,57 @@
+/-
+ Copyright Cedar Contributors
+
+ Licensed under the Apache License, Version 2.0 (the "License");
+ you may not use this file except in compliance with the License.
+ You may obtain a copy of the License at
+
+      https://www.apache.org/licenses/LICENSE-2.0
+
+ Unless required by applicable law or agreed to in writing, software
+ distributed under the License is distributed on an "AS IS" BASIS,
+ WITHOUT WARRANTIES OR CONDITIONS OF ANY KIND, either express or implied.
+ See the License for the specific language governing permissions and
+ limitations under the License.
+-/
+
+import Cedar.Partial.Evaluator
+import Cedar.Spec.Evaluator
+import Cedar.Thm.Data.Control
+import Cedar.Thm.Partial.Evaluation.Basic
+
+namespace Cedar.Thm.Partial.Evaluation.And
+
+open Cedar.Data
+open Cedar.Spec (Result)
+
+/--
+  Inductive argument that partial evaluating a concrete `Partial.Expr.and`
+  expression gives the same output as concrete-evaluating the `Spec.Expr.and`
+  with the same subexpressions
+-/
+theorem on_concrete_eqv_concrete_eval {x₁ x₂ : Spec.Expr} {request : Spec.Request} {entities : Spec.Entities} :
+  Partial.evaluate x₁ request entities = (Spec.evaluate x₁ request entities).map Partial.Value.value →
+  Partial.evaluate x₂ request entities = (Spec.evaluate x₂ request entities).map Partial.Value.value →
+  Partial.evaluate (Partial.Expr.and x₁ x₂) request entities = (Spec.evaluate (Spec.Expr.and x₁ x₂) request entities).map Partial.Value.value
+:= by
+  intro ih₁ ih₂
+  unfold Partial.evaluate Spec.evaluate
+  simp only [ih₁, ih₂]
+  simp only [Except.map, pure, Except.pure, Result.as, Coe.coe]
+  cases h₁ : Spec.evaluate x₁ request entities <;> simp only [Bool.not_eq_true', Except.bind_err, Except.bind_ok]
+  case ok v₁ =>
+    simp only [Spec.Value.asBool]
+    cases v₁ <;> try simp only [Except.bind_err]
+    case prim p =>
+      cases p <;> simp only [Except.bind_ok, Except.bind_err]
+      case bool b =>
+        cases b <;> simp only [ite_true, ite_false]
+        case true =>
+          split <;> simp only [Except.bind_ok, Except.bind_err]
+          case h_1 e h₂ => simp only [h₂, Except.bind_err]
+          case h_2 v h₂ =>
+            simp only [h₂]
+            cases v <;> try simp only [Except.bind_err]
+            case prim p => cases p <;> simp
+
+end Cedar.Thm.Partial.Evaluation.And
