cedar-lean/Cedar/Thm/Partial/Evaluation/Basic.lean
@@ -1,0 +1,80 @@
+/-
+ Copyright Cedar Contributors
+
+ Licensed under the Apache License, Version 2.0 (the "License");
+ you may not use this file except in compliance with the License.
+ You may obtain a copy of the License at
+
+      https://www.apache.org/licenses/LICENSE-2.0
+
+ Unless required by applicable law or agreed to in writing, software
+ distributed under the License is distributed on an "AS IS" BASIS,
+ WITHOUT WARRANTIES OR CONDITIONS OF ANY KIND, either express or implied.
+ See the License for the specific language governing permissions and
+ limitations under the License.
+-/
+
+import Cedar.Partial.Entities
+import Cedar.Partial.Request
+import Cedar.Partial.Value
+import Cedar.Spec.Request
+import Cedar.Spec.Value
+import Cedar.Thm.Data.Map
+import Cedar.Thm.Data.Set
+
+/-!
+  This file contains definitions used by multiple files in the Thm/Partial
+  folder
+-/
+
+namespace Cedar.Spec
+
+/--
+  We define `WellFormed` for `Value` in the obvious way
+-/
+def Value.WellFormed (v : Value) : Prop :=
+  match v with
+  | .set s => s.WellFormed
+  | .record r => r.WellFormed
+  | _ => true
+
+/--
+  `Request`s are `WellFormed` if the context is `WellFormed`
+-/
+def Request.WellFormed (req : Request) : Prop :=
+  req.context.WellFormed
+
+end Cedar.Spec
+
+namespace Cedar.Partial
+
+/--
+  We define `WellFormed` for `Partial.Value` using `Spec.Value.WellFormed`
+-/
+def Value.WellFormed (pval : Partial.Value) : Prop :=
+  match pval with
+  | .value v => v.WellFormed
+  | .residual _ => true
+
+/--
+  `Partial.Request`s are `AllWellFormed` if the context is `WellFormed` and
+  all the context's constituent `Partial.RestrictedValue`s are also `WellFormed`.
+  (principal, action, and resource are always well-formed)
+-/
+def Request.AllWellFormed (preq : Partial.Request) : Prop :=
+  preq.context.WellFormed ∧ ∀ rpval ∈ preq.context.values, rpval.WellFormed
+
+/--
+  We define `WellFormed` for `Partial.EntityData` in the obvious way
+-/
+def EntityData.WellFormed (edata : Partial.EntityData) : Prop :=
+  edata.attrs.WellFormed ∧ edata.ancestors.WellFormed
+
+/--
+  `Partial.Entities` are `AllWellFormed` if they are `WellFormed` and all the
+  constituent `Partial.EntityData` are also `WellFormed`
+-/
+def Entities.AllWellFormed (entities : Partial.Entities) : Prop :=
+  entities.WellFormed ∧ ∀ edata ∈ entities.values, edata.WellFormed
+
+end Cedar.Partial
