cedar-lean/Cedar/Thm/Partial/Evaluation/Call.lean
@@ -1,0 +1,58 @@
+/-
+ Copyright Cedar Contributors
+
+ Licensed under the Apache License, Version 2.0 (the "License");
+ you may not use this file except in compliance with the License.
+ You may obtain a copy of the License at
+
+      https://www.apache.org/licenses/LICENSE-2.0
+
+ Unless required by applicable law or agreed to in writing, software
+ distributed under the License is distributed on an "AS IS" BASIS,
+ WITHOUT WARRANTIES OR CONDITIONS OF ANY KIND, either express or implied.
+ See the License for the specific language governing permissions and
+ limitations under the License.
+-/
+
+import Cedar.Partial.Evaluator
+import Cedar.Spec.Evaluator
+import Cedar.Thm.Data.Control
+import Cedar.Thm.Data.List
+import Cedar.Thm.Partial.Evaluation.Set
+
+namespace Cedar.Thm.Partial.Evaluation.Call
+
+open Cedar.Spec (Error ExtFun Result)
+
+/--
+  `Partial.evaluateCall` on concrete arguments gives the same output as
+  `Spec.call` on those same arguments
+-/
+theorem evaluateCall_on_concrete_eqv_concrete {vs : List Spec.Value} {xfn : ExtFun} :
+  Partial.evaluateCall xfn (vs.map Partial.Value.value) = (Spec.call xfn vs).map Partial.Value.value
+:= by
+  unfold Partial.evaluateCall
+  simp only [List.mapM_map, List.mapM_some, Except.map]
+  cases Spec.call xfn vs <;> simp
+
+/--
+  Inductive argument that partial evaluating a concrete `Partial.Expr.call`
+  expression gives the same output as concrete-evaluating the `Spec.Expr.call`
+  with the same subexpressions
+-/
+theorem on_concrete_eqv_concrete_eval {xs : List Spec.Expr} {request : Spec.Request} {entities : Spec.Entities} {xfn : ExtFun} :
+  (∀ x ∈ xs, Partial.evaluate x request entities = (Spec.evaluate x request entities).map Partial.Value.value) →
+  Partial.evaluate (Partial.Expr.call xfn (xs.map₁ λ x => Spec.Expr.asPartialExpr x.val)) request entities = (Spec.evaluate (Spec.Expr.call xfn xs) request entities).map Partial.Value.value
+:= by
+  intro ih₁
+  unfold Partial.evaluate Spec.evaluate
+  rw [List.map₁_eq_map Spec.Expr.asPartialExpr]
+  rw [List.mapM₁_eq_mapM (Partial.evaluate · request entities)]
+  rw [List.mapM₁_eq_mapM (Spec.evaluate · request entities)]
+  rw [List.mapM_map]
+  rw [Set.mapM_partial_eval_eqv_concrete_eval ih₁]
+  cases xs.mapM (Spec.evaluate · request entities) <;> simp only [Except.bind_ok, Except.bind_err]
+  case error e => simp [Except.map]
+  case ok vs => exact evaluateCall_on_concrete_eqv_concrete
+
+end Cedar.Thm.Partial.Evaluation.Call
