cedar-lean/Cedar/Thm/Partial/Evaluation/GetAttr.lean
@@ -1,0 +1,125 @@
+/-
+ Copyright Cedar Contributors
+
+ Licensed under the Apache License, Version 2.0 (the "License");
+ you may not use this file except in compliance with the License.
+ You may obtain a copy of the License at
+
+      https://www.apache.org/licenses/LICENSE-2.0
+
+ Unless required by applicable law or agreed to in writing, software
+ distributed under the License is distributed on an "AS IS" BASIS,
+ WITHOUT WARRANTIES OR CONDITIONS OF ANY KIND, either express or implied.
+ See the License for the specific language governing permissions and
+ limitations under the License.
+-/
+
+import Cedar.Partial.Evaluator
+import Cedar.Spec.Evaluator
+import Cedar.Thm.Data.Control
+import Cedar.Thm.Data.Map
+import Cedar.Thm.Data.Set
+import Cedar.Thm.Partial.Evaluation.Basic
+
+namespace Cedar.Thm.Partial.Evaluation.GetAttr
+
+open Cedar.Data
+open Cedar.Spec (Attr EntityUID Error Result)
+
+/--
+  if `entities.attrs uid` is `ok` with some attrs, those attrs are a
+  well-formed `Map`
+-/
+theorem partialEntities_attrs_wf {entities : Partial.Entities} {uid : EntityUID} {attrs: Map String Partial.Value} :
+  entities.AllWellFormed →
+  entities.attrs uid = .ok attrs →
+  attrs.WellFormed
+:= by
+  unfold Partial.Entities.attrs Partial.Entities.AllWellFormed Partial.EntityData.WellFormed
+  intro wf h₁
+  cases h₂ : entities.findOrErr uid Error.entityDoesNotExist
+  <;> simp only [h₂, Except.bind_err, Except.bind_ok, Except.ok.injEq] at h₁
+  case ok attrs =>
+    subst h₁
+    have ⟨wf_m, wf_edata⟩ := wf ; clear wf
+    apply (wf_edata _ _).left
+    have h₃ := Map.in_values_iff_findOrErr_ok (v := attrs) (e := Error.entityDoesNotExist) wf_m
+    simp only [h₃]
+    exists uid
+
+/--
+  if `Partial.attrsOf` returns `ok` with some attrs, those attrs are a
+  well-formed `Map`
+-/
+theorem attrsOf_wf {entities : Partial.Entities} {v : Spec.Value} {attrs : Map String Partial.Value} :
+  entities.AllWellFormed →
+  v.WellFormed →
+  Partial.attrsOf v entities.attrs = .ok attrs →
+  attrs.WellFormed
+:= by
+  intro wf_e wf_v
+  unfold Partial.attrsOf
+  cases v <;> try simp only [false_implies, Except.ok.injEq]
+  case prim p =>
+    cases p <;> simp only [false_implies]
+    case entityUID uid => exact partialEntities_attrs_wf wf_e
+  case record r =>
+    intro h₁
+    subst h₁
+    apply Map.mapOnValues_wf.mp wf_v
+
+/--
+  `Partial.attrsOf` on concrete arguments is the same as `Spec.attrsOf` on those
+  arguments
+-/
+theorem attrsOf_on_concrete_eqv_concrete {v : Spec.Value} {entities : Spec.Entities} :
+  Partial.attrsOf v (Partial.Entities.attrs entities) = (Spec.attrsOf v (Spec.Entities.attrs entities)).map λ m => m.mapOnValues Partial.Value.value
+:= by
+  unfold Partial.attrsOf Spec.attrsOf Except.map
+  cases v <;> simp only
+  case prim p =>
+    cases p <;> simp only
+    case entityUID uid =>
+      unfold Partial.Entities.attrs Spec.Entities.attrs Spec.Entities.asPartialEntities
+      cases h₁ : entities.findOrErr uid Error.entityDoesNotExist
+      <;> simp [h₁, Map.findOrErr_mapOnValues, Except.map, Spec.EntityData.asPartialEntityData]
+
+/--
+  `Partial.getAttr` on concrete arguments is the same as `Spec.getAttr` on those
+  arguments
+-/
+theorem getAttr_on_concrete_eqv_concrete {v : Spec.Value} {entities : Spec.Entities} {attr : Attr} :
+  Partial.getAttr v attr entities = (Spec.getAttr v attr entities).map Partial.Value.value
+:= by
+  unfold Partial.getAttr Spec.getAttr
+  simp only [attrsOf_on_concrete_eqv_concrete, Except.map]
+  cases Spec.attrsOf v entities.attrs <;> simp only [Except.bind_err, Except.bind_ok]
+  case ok m => simp [Map.findOrErr_mapOnValues, Except.map]
+
+/--
+  `Partial.evaluateGetAttr` on concrete arguments is the same as `Spec.getAttr`
+  on those arguments
+-/
+theorem evaluateGetAttr_on_concrete_eqv_concrete {v : Spec.Value} {a : Attr} {entities : Spec.Entities} :
+  Partial.evaluateGetAttr v a entities = Spec.getAttr v a entities
+:= by
+  simp only [Partial.evaluateGetAttr, getAttr_on_concrete_eqv_concrete, pure, Except.pure, Except.map]
+  cases h : Spec.getAttr v a entities <;> simp [h]
+
+/--
+  Inductive argument that partial evaluating a concrete `Partial.Expr.getAttr`
+  expression gives the same output as concrete-evaluating the
+  `Spec.Expr.getAttr` with the same subexpressions
+-/
+theorem on_concrete_eqv_concrete_eval {x₁ : Spec.Expr} {request : Spec.Request} {entities : Spec.Entities} {attr : Attr} :
+  Partial.evaluate x₁ request entities = (Spec.evaluate x₁ request entities).map Partial.Value.value →
+  Partial.evaluate (Partial.Expr.getAttr x₁ attr) request entities = (Spec.evaluate (Spec.Expr.getAttr x₁ attr) request entities).map Partial.Value.value
+:= by
+  intro ih₁
+  unfold Partial.evaluate Spec.evaluate
+  simp only [ih₁]
+  cases Spec.evaluate x₁ request entities <;> simp only [Except.bind_err, Except.bind_ok]
+  case error e => simp [Except.map]
+  case ok v₁ => exact evaluateGetAttr_on_concrete_eqv_concrete
+
+end Cedar.Thm.Partial.Evaluation.GetAttr
