cedar-lean/Cedar/Thm/Partial/Evaluation/HasAttr.lean
@@ -1,0 +1,99 @@
+/-
+ Copyright Cedar Contributors
+
+ Licensed under the Apache License, Version 2.0 (the "License");
+ you may not use this file except in compliance with the License.
+ You may obtain a copy of the License at
+
+      https://www.apache.org/licenses/LICENSE-2.0
+
+ Unless required by applicable law or agreed to in writing, software
+ distributed under the License is distributed on an "AS IS" BASIS,
+ WITHOUT WARRANTIES OR CONDITIONS OF ANY KIND, either express or implied.
+ See the License for the specific language governing permissions and
+ limitations under the License.
+-/
+
+import Cedar.Partial.Evaluator
+import Cedar.Spec.Evaluator
+import Cedar.Thm.Data.Control
+import Cedar.Thm.Data.Map
+import Cedar.Thm.Data.Set
+import Cedar.Thm.Partial.Evaluation.Basic
+
+namespace Cedar.Thm.Partial.Evaluation.HasAttr
+
+open Cedar.Data
+open Cedar.Spec (Attr Error Result)
+
+/--
+  `Partial.attrsOf` on concrete arguments is the same as `Spec.attrsOf` on those
+  arguments
+
+  Note that the "concrete arguments" provided to `Partial.attrsOf` and
+  `Spec.attrsOf` in this theorem are different from the "concrete arguments"
+  provided in the theorem of the same name in Partial/Evaluation/GetAttr.lean
+-/
+theorem Partial.attrsOf_on_concrete_eqv_attrsOf {v : Spec.Value} {entities : Spec.Entities} :
+  Partial.attrsOf v (λ uid => .ok (entities.asPartialEntities.attrsOrEmpty uid)) =
+  (Spec.attrsOf v (λ uid => .ok (entities.attrsOrEmpty uid))).map λ m => m.mapOnValues Partial.Value.value
+:= by
+  unfold Partial.attrsOf Spec.attrsOf Except.map
+  cases v <;> simp only
+  case prim p =>
+    cases p <;> simp only
+    case entityUID uid =>
+      unfold Partial.Entities.attrsOrEmpty Spec.Entities.attrsOrEmpty Spec.Entities.asPartialEntities
+      cases h₁ : (entities.mapOnValues Spec.EntityData.asPartialEntityData).find? uid
+      <;> simp only [Except.ok.injEq]
+      <;> cases h₂ : entities.find? uid <;> simp only
+      <;> unfold Spec.EntityData.asPartialEntityData at h₁
+      <;> simp only [← Map.find?_mapOnValues, Option.map_eq_none', Option.map_eq_some'] at h₁
+      case none.none => simp [Map.mapOnValues_empty]
+      case none.some => simp [h₁] at h₂
+      case some.none => simp [h₂] at h₁
+      case some.some edata₁ edata₂ =>
+        replace ⟨edata₁, ⟨h₁, h₃⟩⟩ := h₁
+        simp only [h₂, Option.some.injEq] at h₁
+        subst h₁ h₃
+        simp [Map.mapOnValues]
+
+/--
+  `Partial.hasAttr` on concrete arguments is the same as `Spec.hasAttr` on those
+  arguments
+-/
+theorem Partial.hasAttr_on_concrete_eqv_hasAttr {v : Spec.Value} {entities : Spec.Entities} {attr : Attr} :
+  Partial.hasAttr v attr entities = Spec.hasAttr v attr entities
+:= by
+  unfold Partial.hasAttr Spec.hasAttr
+  simp only [Partial.attrsOf_on_concrete_eqv_attrsOf, Except.map]
+  cases Spec.attrsOf v λ uid => .ok (entities.attrsOrEmpty uid)
+  <;> simp only [Except.bind_ok, Except.bind_err, Except.ok.injEq, Spec.Value.prim.injEq, Spec.Prim.bool.injEq]
+  case ok m => simp [← Map.mapOnValues_contains]
+
+/--
+  `Partial.evaluateHasAttr` on concrete arguments is the same as `Spec.hasAttr`
+  on those arguments
+-/
+theorem Partial.evaluateHasAttr_on_concrete_eqv_hasAttr {v : Spec.Value} {a : Attr} {entities : Spec.Entities} :
+  Partial.evaluateHasAttr v a entities = Spec.hasAttr v a entities
+:= by
+  simp [Partial.evaluateHasAttr, Partial.hasAttr_on_concrete_eqv_hasAttr, pure, Except.pure]
+
+/--
+  Inductive argument that partial evaluating a concrete `Partial.Expr.hasAttr`
+  expression gives the same output as concrete-evaluating the
+  `Spec.Expr.hasAttr` with the same subexpressions
+-/
+theorem on_concrete_eqv_concrete_eval {x₁ : Spec.Expr} {request : Spec.Request} {entities : Spec.Entities} {attr : Attr} :
+  Partial.evaluate x₁ request entities = (Spec.evaluate x₁ request entities).map Partial.Value.value →
+  Partial.evaluate (Partial.Expr.hasAttr x₁ attr) request entities = (Spec.evaluate (Spec.Expr.hasAttr x₁ attr) request entities).map Partial.Value.value
+:= by
+  intro ih₁
+  unfold Partial.evaluate Spec.evaluate
+  simp only [ih₁]
+  cases Spec.evaluate x₁ request entities <;> simp only [Except.bind_err, Except.bind_ok]
+  case error e => simp [Except.map]
+  case ok v₁ => exact Partial.evaluateHasAttr_on_concrete_eqv_hasAttr
+
+end Cedar.Thm.Partial.Evaluation.HasAttr
