cedar-lean/Cedar/Thm/Partial/Evaluation/Set.lean
@@ -1,0 +1,87 @@
+/-
+ Copyright Cedar Contributors
+
+ Licensed under the Apache License, Version 2.0 (the "License");
+ you may not use this file except in compliance with the License.
+ You may obtain a copy of the License at
+
+      https://www.apache.org/licenses/LICENSE-2.0
+
+ Unless required by applicable law or agreed to in writing, software
+ distributed under the License is distributed on an "AS IS" BASIS,
+ WITHOUT WARRANTIES OR CONDITIONS OF ANY KIND, either express or implied.
+ See the License for the specific language governing permissions and
+ limitations under the License.
+-/
+
+import Cedar.Partial.Evaluator
+import Cedar.Spec.Policy
+import Cedar.Thm.Data.Control
+import Cedar.Thm.Data.List
+import Cedar.Thm.Data.Set
+import Cedar.Thm.Partial.Evaluation.Basic
+
+namespace Cedar.Thm.Partial.Evaluation.Set
+
+open Cedar.Data
+open Cedar.Spec (Result)
+
+/--
+  Lemma (used for both the Set and Call cases):
+
+  Inductive argument that `mapM`'ing partial evaluation over a list of concrete
+  exprs gives the same output as `mapM`'ing concrete evaluation over the same
+  exprs
+-/
+theorem mapM_partial_eval_eqv_concrete_eval {xs : List Spec.Expr} {request : Spec.Request} {entities : Spec.Entities} :
+  (∀ x ∈ xs, Partial.evaluate x request entities = (Spec.evaluate x request entities).map Partial.Value.value) →
+  xs.mapM (λ x => Partial.evaluate x.asPartialExpr request entities) = (xs.mapM (Spec.evaluate · request entities)).map λ vs => vs.map Partial.Value.value
+:= by
+  intro ih₁
+  induction xs
+  case nil => simp [Except.map, pure, Except.pure]
+  case cons hd tl ih =>
+    specialize ih (by
+      intro x' h₁
+      exact ih₁ x' (List.mem_cons_of_mem hd h₁)
+    )
+    cases h₁ : Spec.evaluate hd request entities
+    <;> cases h₂ : Partial.evaluate hd request entities
+    <;> simp only [h₁, h₂, List.mapM_cons, Except.bind_err, Except.bind_ok]
+    case error.error e₁ e₂ =>
+      simp only [ih₁ hd, h₁, Except.map, List.mem_cons, true_or, Except.error.injEq] at h₂
+      simp [h₂, Except.map]
+    case ok.error val e | error.ok e pval =>
+      simp [ih₁ hd, h₁, Except.map] at h₂
+    case ok.ok val pval =>
+      simp only [ih₁, h₁, Except.map, List.mem_cons, true_or, Except.ok.injEq] at h₂
+      subst h₂
+      -- the remaining goal is just a statement about `tl`, not `hd` itself
+      -- so we can dispatch it using `ih`
+      generalize h₃ : (tl.mapM λ x => Partial.evaluate x.asPartialExpr request entities) = pres at *
+      generalize h₄ : (tl.mapM λ x => Spec.evaluate x request entities) = sres at *
+      cases pres <;> cases sres
+      <;> simp only [Except.map, pure, Except.pure, List.mem_cons, Except.error.injEq, Except.ok.injEq, Except.bind_ok, Except.bind_err, List.cons.injEq, List.map_cons, forall_eq_or_imp, true_and] at *
+      case error.error e₁ e₂ => exact ih
+      case ok.ok pvals vals => exact ih
+
+/--
+  Inductive argument that partial evaluating a concrete `Partial.Expr.set`
+  expression gives the same output as concrete-evaluating the `Spec.Expr.set`
+  with the same subexpressions
+-/
+theorem on_concrete_eqv_concrete_eval {xs : List Spec.Expr} {request : Spec.Request} {entities : Spec.Entities} :
+  (∀ x ∈ xs, Partial.evaluate x request entities = (Spec.evaluate x request entities).map Partial.Value.value) →
+  Partial.evaluate (Partial.Expr.set (xs.map₁ λ x => Spec.Expr.asPartialExpr x.val)) request entities = (Spec.evaluate (Spec.Expr.set xs) request entities).map Partial.Value.value
+:= by
+  intro ih₁
+  unfold Partial.evaluate Spec.evaluate
+  rw [List.map₁_eq_map Spec.Expr.asPartialExpr]
+  rw [List.mapM₁_eq_mapM (Partial.evaluate · request entities)]
+  rw [List.mapM₁_eq_mapM (Spec.evaluate · request entities)]
+  rw [List.mapM_map]
+  rw [mapM_partial_eval_eqv_concrete_eval ih₁]
+  cases xs.mapM (Spec.evaluate · request entities) <;> simp only [Except.map, Except.bind_err, Except.bind_ok]
+  case ok vs => simp [List.mapM_map, List.mapM_some]
+
+end Cedar.Thm.Partial.Evaluation.Set
