cedar-lean/Cedar/Thm/Partial/Evaluation/Unary.lean
@@ -1,0 +1,51 @@
+/-
+ Copyright Cedar Contributors
+
+ Licensed under the Apache License, Version 2.0 (the "License");
+ you may not use this file except in compliance with the License.
+ You may obtain a copy of the License at
+
+      https://www.apache.org/licenses/LICENSE-2.0
+
+ Unless required by applicable law or agreed to in writing, software
+ distributed under the License is distributed on an "AS IS" BASIS,
+ WITHOUT WARRANTIES OR CONDITIONS OF ANY KIND, either express or implied.
+ See the License for the specific language governing permissions and
+ limitations under the License.
+-/
+
+import Cedar.Partial.Evaluator
+import Cedar.Spec.Evaluator
+import Cedar.Thm.Data.Control
+import Cedar.Thm.Partial.Evaluation.Basic
+
+namespace Cedar.Thm.Partial.Evaluation.Unary
+
+open Cedar.Spec (UnaryOp)
+
+/--
+  `Partial.apply₁` on concrete arguments gives the same output as `Spec.apply₁`
+  on the same arguments
+-/
+theorem apply₁_on_concrete_eqv_concrete {op : UnaryOp} {v : Spec.Value} :
+  Partial.apply₁ op v = (Spec.apply₁ op v).map Partial.Value.value
+:= by
+  rfl
+
+/--
+  Inductive argument that partial evaluating a concrete `Partial.Expr.unaryApp`
+  expression gives the same output as concrete-evaluating the
+  `Spec.Expr.unaryApp` with the same subexpressions
+-/
+theorem on_concrete_eqv_concrete_eval {x₁ : Spec.Expr} {request : Spec.Request} {entities : Spec.Entities} {op : UnaryOp} :
+  Partial.evaluate x₁ request entities = (Spec.evaluate x₁ request entities).map Partial.Value.value →
+  Partial.evaluate (Partial.Expr.unaryApp op x₁) request entities = (Spec.evaluate (Spec.Expr.unaryApp op x₁) request entities).map Partial.Value.value
+:= by
+  intro ih₁
+  unfold Partial.evaluate Spec.evaluate
+  simp only [ih₁]
+  cases Spec.evaluate x₁ request entities <;> simp only [Except.bind_err, Except.bind_ok]
+  case error e => simp [Except.map]
+  case ok v₁ => rfl
+
+end Cedar.Thm.Partial.Evaluation.Unary
